Define some processor platforms

schedule.v
@@ -1,29 +1,66 @@
 Add LoadPath "/home/felipec/dev/coq/rt-scheduling-spec".
 Require Import job.
 Require Import Coq.Lists.ListSet.
+Require Import Coq.Lists.List.
 
 Definition time := nat.
 
 Axiom schedule : Set.
-Axiom scheduled : task -> schedule -> nat -> Prop.
+(*Axiom scheduled : task -> schedule -> nat -> Prop.*)
 Axiom exec : task -> schedule -> nat -> nat.
 
 Definition cpu_platform := Set.
-Axiom cpuset : schedule -> cpu_platform.
+Axiom platform_of : schedule -> cpu_platform.
 
 Record ident_mp (platform: cpu_platform) (num_cpus: nat) : Prop :=
-  { maximum_cpus: forall (s: schedule) (t: time),
-           cpuset s = platform ->
-               (exists (l: list task),
+  { ident_mp_maximum_exec: forall (tsk: task) (s: schedule) (t: time),
+           platform_of s = platform -> exec tsk s t <= 1;
+    ident_mp_mapping: forall (s: schedule) (t: time),
+           platform_of s = platform ->
+               (exists !(l: list task),
                    length l < num_cpus /\
                    forall (tsk: task),
-                       List.In tsk l <-> scheduled tsk s t)
+                       List.In tsk l <-> exec tsk s t = 1)
   }.
 
-Axiom 
+Record unif_mp (platform: cpu_platform) (total_speed: nat) (max_speed: nat) : Prop :=
+  { unif_mp_maximum_speed: forall (tsk: task) (s: schedule) (t: time),
+          platform_of s = platform -> exec tsk s t <= max_speed;
+    unif_mp_cumulative_speed:
+          let exec2 (s: schedule) (t: time) (tsk:task) : nat := exec tsk s t in
+              forall (s: schedule) (t: time),
+                  platform_of s = platform ->
+                      (exists ! (l: list task),
+                          (forall (tsk: task), List.In tsk l <-> exec tsk s t > 0)
+                          /\ (fold_left plus (map (exec2 s t) l) 0) <= total_speed)
+  }.
+
+Axiom cpu_list : cpu_platform -> list nat.
+Axiom affinity : task -> cpu_platform -> list nat.
+
+Record apa_ident_mp (platform: cpu_platform) (num_cpus: nat) : Prop :=
+  { apa_ident_is_ident: ident_mp platform num_cpus;
+    restricted_affinities:
+        forall (s: schedule) (t: time),
+            platform_of s = platform ->
+            (forall (l: list task) (tsk: task) (cpu: nat),
+                exec tsk s t = 1 ->
+                cpu < num_cpus ->
+                (nth cpu l tsk = tsk) ->
+                List.In cpu (affinity tsk platform))
+  }.
 
 Fixpoint service (tsk: task) (s: schedule) (t: time) : nat:=
   match t with
-  | 0=> 0
-  | Sn=> 1
+  | 0 => exec tsk s 0
+  | S n => service tsk s n + exec tsk s (S n)
   end.
+
+Lemma exists_global_apa_platform :
+    forall (platform: cpu_platform) (num_cpus: nat) (s: schedule),
+        ident_mp platform num_cpus ->
+        platform_of s = platform ->
+        exists (platform': cpu_platform) (s': schedule),
+            apa_ident_mp platform' num_cpus
+            /\ platform_of s' = platform'.
+            (*/\ (forall t: time, service tsk s t = service tsk s' t).*)
